src/Prototype/SingleValue.v
@@ -70,6 +70,9 @@ Section Impl.
   Definition parentIdx := 0.
   Definition child1Idx := 1.
   Definition child2Idx := 2.
+  Definition implIndices := parentIdx :: child1Idx :: child2Idx :: nil.
+  Definition from_external (i: IdxT) :=
+    if in_dec eq_nat_dec i implIndices then false else true.
 
   Definition theOtherChild (idx: nat) :=
     if eq_nat_dec idx child1Idx then child2Idx else child1Idx.
@@ -80,63 +83,69 @@ Section Impl.
 
     Definition ParentGetReq : RuleT SingleValueMsg ParentState :=
       fun msg =>
-        match msg_content msg with
-        | SvmGetReq =>
-          fun st =>
-            match ps_request_from st with
-            | Some _ => None
-            | None => if ps_is_valid st
-                      then Some ((buildMsg Resp parentIdx (msg_from msg)
-                                           (SvmGetResp (ps_value st))) :: nil,
-                                 {| ps_is_valid := false;
-                                    ps_value := ps_value st;
-                                    ps_request_from := ps_request_from st |})
-                      else Some ((buildMsg Req parentIdx (theOtherChild (msg_from msg))
-                                           SvmInvReq) :: nil,
-                                 {| ps_is_valid := ps_is_valid st;
-                                    ps_value := ps_value st;
-                                    ps_request_from := Some (msg_from msg, true) |})
-            end
-        | _ => fun _ => None
-        end.
+        if from_external (msg_from msg) then fun _ => None
+        else
+          match msg_content msg with
+          | SvmGetReq =>
+            fun st =>
+              match ps_request_from st with
+              | Some _ => None
+              | None => if ps_is_valid st
+                        then Some ((buildMsg Resp parentIdx (msg_from msg)
+                                             (SvmGetResp (ps_value st))) :: nil,
+                                   {| ps_is_valid := false;
+                                      ps_value := ps_value st;
+                                      ps_request_from := ps_request_from st |})
+                        else Some ((buildMsg Req parentIdx (theOtherChild (msg_from msg))
+                                             SvmInvReq) :: nil,
+                                   {| ps_is_valid := ps_is_valid st;
+                                      ps_value := ps_value st;
+                                      ps_request_from := Some (msg_from msg, true) |})
+              end
+          | _ => fun _ => None
+          end.
 
     Definition ParentSetReq : RuleT SingleValueMsg ParentState :=
       fun msg =>
-        match msg_content msg with
-        | SvmSetReq _ =>
-          fun st =>
-            match ps_request_from st with
-            | Some _ => None
-            | None => if ps_is_valid st
-                      then Some ((buildMsg Resp parentIdx (msg_from msg) SvmSetResp) :: nil,
-                                 {| ps_is_valid := false;
-                                    ps_value := ps_value st;
-                                    ps_request_from := ps_request_from st |})
-                      else Some ((buildMsg Req parentIdx (theOtherChild (msg_from msg))
-                                           SvmInvReq) :: nil,
-                                 {| ps_is_valid := ps_is_valid st;
-                                    ps_value := ps_value st;
-                                    ps_request_from := Some (msg_from msg, false) |})
-            end
-        | _ => fun _ => None
-        end.
+        if from_external (msg_from msg) then fun _ => None
+        else
+          match msg_content msg with
+          | SvmSetReq _ =>
+            fun st =>
+              match ps_request_from st with
+              | Some _ => None
+              | None => if ps_is_valid st
+                        then Some ((buildMsg Resp parentIdx (msg_from msg) SvmSetResp) :: nil,
+                                   {| ps_is_valid := false;
+                                      ps_value := ps_value st;
+                                      ps_request_from := ps_request_from st |})
+                        else Some ((buildMsg Req parentIdx (theOtherChild (msg_from msg))
+                                             SvmInvReq) :: nil,
+                                   {| ps_is_valid := ps_is_valid st;
+                                      ps_value := ps_value st;
+                                      ps_request_from := Some (msg_from msg, false) |})
+              end
+          | _ => fun _ => None
+          end.
 
     Definition ParentInvResp : RuleT SingleValueMsg ParentState :=
       fun msg =>
-        match msg_content msg with
-        | SvmInvResp v =>
-          fun st =>
-            match ps_request_from st with
-            | None => None
-            | Some (childTo, is_get) =>
-              Some ((buildMsg Resp parentIdx childTo
-                              (if is_get then SvmGetResp v else SvmSetResp)) :: nil,
-                    {| ps_is_valid := ps_is_valid st;
-                       ps_value := ps_value st;
-                       ps_request_from := None |})
-            end
-        | _ => fun _ => None
-        end.
+        if from_external (msg_from msg) then fun _ => None
+        else
+          match msg_content msg with
+          | SvmInvResp v =>
+            fun st =>
+              match ps_request_from st with
+              | None => None
+              | Some (childTo, is_get) =>
+                Some ((buildMsg Resp parentIdx childTo
+                                (if is_get then SvmGetResp v else SvmSetResp)) :: nil,
+                      {| ps_is_valid := ps_is_valid st;
+                         ps_value := ps_value st;
+                         ps_request_from := None |})
+              end
+          | _ => fun _ => None
+          end.
 
     Definition parent : Object SingleValueMsg ParentState :=
       {| obj_idx := parentIdx;
@@ -153,97 +162,107 @@ Section Impl.
     (* from external *)
     Definition ChildGetReq : RuleT SingleValueMsg ChildState :=
       fun msg =>
-        match msg_content msg with
-        | SvmGetReq =>
-          fun st =>
-            match cs_request_from st with
-            | Some _ => None
-            | None =>
-              if cs_is_valid st
-              then Some ((buildMsg Resp childIdx (msg_from msg)
-                                   (SvmGetResp (cs_value st))) :: nil,
-                         st)
-              else Some ((buildMsg Req childIdx parentIdx SvmGetReq) :: nil,
-                         {| cs_is_valid := cs_is_valid st;
-                            cs_value := cs_value st;
-                            cs_request_from := Some (msg_from msg, O) |})
-            end
-        | _ => fun _ => None
-        end.
+        if from_external (msg_from msg) then
+          match msg_content msg with
+          | SvmGetReq =>
+            fun st =>
+              match cs_request_from st with
+              | Some _ => None
+              | None =>
+                if cs_is_valid st
+                then Some ((buildMsg Resp childIdx (msg_from msg)
+                                     (SvmGetResp (cs_value st))) :: nil,
+                           st)
+                else Some ((buildMsg Req childIdx parentIdx SvmGetReq) :: nil,
+                           {| cs_is_valid := cs_is_valid st;
+                              cs_value := cs_value st;
+                              cs_request_from := Some (msg_from msg, O) |})
+              end
+          | _ => fun _ => None
+          end
+        else fun _ => None.
 
     (* from the parent *)
     Definition ChildGetResp : RuleT SingleValueMsg ChildState :=
       fun msg =>
-        match msg_content msg with
-        | SvmGetResp v =>
-          fun st =>
-            match cs_request_from st with
-            | None => None
-            | Some (efrom, _) =>
-              Some ((buildMsg Resp childIdx efrom (SvmGetResp v)) :: nil,
-                    {| cs_is_valid := true;
-                       cs_value := v;
-                       cs_request_from := None |})
-            end
-        | _ => fun _ => None
-        end.
+        if from_external (msg_from msg) then fun _ => None
+        else
+          match msg_content msg with
+          | SvmGetResp v =>
+            fun st =>
+              match cs_request_from st with
+              | None => None
+              | Some (efrom, _) =>
+                Some ((buildMsg Resp childIdx efrom (SvmGetResp v)) :: nil,
+                      {| cs_is_valid := true;
+                         cs_value := v;
+                         cs_request_from := None |})
+              end
+          | _ => fun _ => None
+          end.
 
     (* from external *)
     Definition ChildSetReq : RuleT SingleValueMsg ChildState :=
       fun msg =>
-        match msg_content msg with
-        | SvmSetReq v =>
-          fun st =>
-            match cs_request_from st with
-            | Some _ => None
-            | None =>
-              if cs_is_valid st
-              then Some ((buildMsg Resp childIdx (msg_from msg)
-                                   SvmSetResp) :: nil,
-                         {| cs_is_valid := cs_is_valid st;
-                            cs_value := v;
-                            cs_request_from := cs_request_from st |})
-              else Some ((buildMsg Req childIdx parentIdx (SvmSetReq v)) :: nil,
-                         {| cs_is_valid := cs_is_valid st;
-                            cs_value := cs_value st;
-                            cs_request_from := Some (msg_from msg, v) |})
-            end
-        | _ => fun _ => None
-        end.
+        if from_external (msg_from msg) then
+          match msg_content msg with
+          | SvmSetReq v =>
+            fun st =>
+              match cs_request_from st with
+              | Some _ => None
+              | None =>
+                if cs_is_valid st
+                then Some ((buildMsg Resp childIdx (msg_from msg)
+                                     SvmSetResp) :: nil,
+                           {| cs_is_valid := cs_is_valid st;
+                              cs_value := v;
+                              cs_request_from := cs_request_from st |})
+                else Some ((buildMsg Req childIdx parentIdx (SvmSetReq v)) :: nil,
+                           {| cs_is_valid := cs_is_valid st;
+                              cs_value := cs_value st;
+                              cs_request_from := Some (msg_from msg, v) |})
+              end
+          | _ => fun _ => None
+          end
+        else fun _ => None.
 
     (* from the parent *)
     Definition ChildSetResp : RuleT SingleValueMsg ChildState :=
       fun msg =>
-        match msg_content msg with
-        | SvmSetResp =>
-          fun st =>
-            match cs_request_from st with
-            | None => None
-            | Some (efrom, v) =>
-              Some ((buildMsg Resp childIdx efrom SvmSetResp) :: nil,
-                    {| cs_is_valid := true;
-                       cs_value := v;
-                       cs_request_from := None |})
-            end
-        | _ => fun _ => None
-        end.
+        if from_external (msg_from msg) then fun _ => None
+        else
+          match msg_content msg with
+          | SvmSetResp =>
+            fun st =>
+              match cs_request_from st with
+              | None => None
+              | Some (efrom, v) =>
+                Some ((buildMsg Resp childIdx efrom SvmSetResp) :: nil,
+                      {| cs_is_valid := true;
+                         cs_value := v;
+                         cs_request_from := None |})
+              end
+          | _ => fun _ => None
+          end.
 
     (* from the parent *)
     Definition ChildInvReq : RuleT SingleValueMsg ChildState :=
       fun msg =>
-        match msg_content msg with
-        | SvmInvReq =>
-          fun st =>
-            match cs_request_from st with
-            | Some _ => None
-            | None => Some ((buildMsg Resp childIdx parentIdx
-                                      (SvmInvResp (cs_value st))) :: nil,
-                            {| cs_is_valid := false;
-                               cs_value := cs_value st;
-                               cs_request_from := cs_request_from st |})
-            end
-        | _ => fun _ => None
-        end.
+        if from_external (msg_from msg) then fun _ => None
+        else
+          match msg_content msg with
+          | SvmInvReq =>
+            fun st =>
+              match cs_request_from st with
+              | Some _ => None
+              | None => Some ((buildMsg Resp childIdx parentIdx
+                                        (SvmInvResp (cs_value st))) :: nil,
+                              {| cs_is_valid := false;
+                                 cs_value := cs_value st;
+                                 cs_request_from := cs_request_from st |})
+              end
+          | _ => fun _ => None
+          end.
 
     Definition child : Object SingleValueMsg ChildState :=
       {| obj_idx := childIdx;
