src/Prototype/Correctness.v
@@ -1,6 +1,28 @@
 Require Import List String Peano_dec.
 Require Import FnMap Language SingleValue.
 
-Theorem impl_linear: Linear impl.
+Ltac inv H := inversion H; subst; clear H.
+Ltac dest_in :=
+  repeat
+    match goal with
+    | [H: In _ _ |- _] => inv H
+    end.
+
+Theorem impl_linear: ExtLinear impl implIndices.
 Proof.
+  apply linear_extLinear.
+  apply linear_local.
+
+  intros; dest_in.
+
+  - (* parent *)
+    admit.
+  - (* child1 *)
+    admit.
+  - (* child2 *)
+    admit.
+  
 Admitted.
+
+
+
